More theorems

universe-types.lean
@@ -1,16 +1,48 @@
 -- All in term mode, for fun
 
-def List.product (as : List α) (bs : List β) : List (α × β) :=
+namespace List
+
+def product (as : List α) (bs : List β) : List (α × β) :=
   as.flatMap fun a => bs.map (a, ·)
 
-theorem List.mem_product {as : List α} {bs : List β} : (a, b) ∈ as.product bs ↔ a ∈ as ∧ b ∈ bs := ⟨
+theorem mem_product {as : List α} {bs : List β} : (a, b) ∈ as.product bs ↔ a ∈ as ∧ b ∈ bs := ⟨
   (fun h =>
-    have ⟨_, ha', h'⟩ := List.mem_flatMap.mp h
-    have ⟨_, hb', h''⟩ := List.mem_map.mp h'
+    have ⟨_, ha', h'⟩ := mem_flatMap.mp h
+    have ⟨_, hb', h''⟩ := mem_map.mp h'
     have ⟨ha'_eq, hb'_eq⟩ := Prod.mk.inj h''
     ⟨ha'_eq ▸ ha', hb'_eq ▸ hb'⟩),
   fun ⟨ha, hb⟩ =>
-    List.mem_flatMap_of_mem ha <| List.mem_map_of_mem hb⟩
+    mem_flatMap_of_mem ha <| mem_map_of_mem hb⟩
+
+theorem product_ne_nil {as : List α} {bs : List β} (ha : as ≠ []) (hb : bs ≠ []) : as.product bs ≠ [] :=
+  have ⟨_a, _as', ha'⟩ := ne_nil_iff_exists_cons.mp ha
+  have ⟨_b, _bs', hb'⟩ := ne_nil_iff_exists_cons.mp hb
+  ha' ▸ hb' ▸ fun h => cons_ne_nil _ _ h
+
+theorem product_eq {as : List α} {bs : List β} :
+    as.product bs = as.flatMap fun a => bs.map (a, ·) :=
+  rfl
+
+theorem product_nil_left {α β} {bs : List β} : product (α := α) [] bs = [] :=
+  rfl
+
+theorem product_nil_right {α β} {as : List α} : product (β := β) as [] = [] :=
+  product_eq ▸ flatMap_eq_nil_iff.mpr fun _ _ => rfl
+
+theorem map_product {as : List α} {bs : List β} {f : α → γ} {g : β → δ} :
+    (as.product bs).map (Prod.map f g) = product (as.map f) (bs.map g) :=
+  match as with
+  | [] => rfl
+  -- | _ :: _, [] => product_nil_right ▸ product_nil_right (as := map f _) ▸ rfl
+  | _ :: _ =>
+    -- product_eq ▸ Eq.symm product_eq ▸ map_flatMap ▸ Eq.symm flatMap_map \t sorry
+    by simp [product, map_flatMap, flatMap_map]; rfl -- TODO
+
+theorem map_product' {as : List α} {bs : List β} {f : (α × β) → γ} :
+  (as.product bs).map f = (as.map (Function.curry f)|>.product bs).map fun (f, b) => f b :=
+  sorry
+
+end List
 
 inductive Finite where
   | unit : Finite
@@ -35,6 +67,13 @@ where
     | .pair l r => (go l, go r)
     | .arrow _ dst => fun _ => go dst
 
+def enumerateArrow {α β : Type} (as : List α) (bs : List β) (beq : α → α → Bool) : List (α → β) :=
+  as.foldr (init := match bs with | [] => [] | b :: _ => [fun _ => b]) -- note this `init` is not correct if `as = []`
+    fun a acc =>
+      (acc.product bs).map fun (oldFn, b) =>
+        fun a' =>
+          if beq a a' then b else oldFn a'
+
 mutual
 def beq (t : Finite) (x y : t.asType) : Bool :=
   match t with
@@ -52,64 +91,225 @@ def enumerate : (t : Finite) → List t.asType
   | .unit => [()]
   | .bool => [true, false]
   | .pair l r => List.product (enumerate l) (enumerate r)
-  | .arrow tα tβ =>
-    let as := enumerate tα
-    let bs := enumerate tβ
-    as.foldr (init := [fun _ => default])
-      fun a acc =>
-        (acc.product bs).map fun (oldFn, b) =>
-          fun a' =>
-            if beq tα a a' then b else oldFn a'
+  | .arrow tα tβ => enumerateArrow (enumerate tα) (enumerate tβ) (beq tα)
 end
 
 instance {t : Finite} : BEq t.asType where
   beq := beq t
 
--- theorem beq_refl : beq t x x = true :=
---   match t with
---   | .unit => rfl
---   | .bool => match x with | true | false => rfl
---   | .pair _ _ => Bool.and_eq_true_iff.mpr ⟨beq_refl, beq_refl⟩
---   | .fn _ _ => List.all_eq_true.mpr fun _ _ => beq_refl
+#eval beq (.arrow (.pair (.arrow .bool .bool) .bool) .bool) (fun (f, x) => f x) (fun (f, x) => f (not x))
 
--- theorem beq.enumerateFn_correct {elts : List α} (h : Complete elts) : Complete (enumerateFn t elts) :=
---   fun f =>
---     match t with
---     | .unit => List.mem_map.mpr ⟨f (), h _, rfl⟩
---     | .bool => List.mem_map.mpr
---       ⟨
---         (f true, f false),
---         List.mem_product.mpr ⟨h _, h _⟩,
---         funext fun | true => rfl | false => rfl⟩
---     | .pair l r => List.mem_map.mpr
---       ⟨
---         Function.curry f,
---         beq.enumerateFn_correct (beq.enumerateFn_correct h) _,
---         Function.uncurry_curry _⟩
---     | .fn src dst => sorry
+theorem enumerateArrow_cons {as : List α} {bs : List β} {eq : α → α → Bool} {a : α} :
+    enumerateArrow (a :: as) bs eq = ((enumerateArrow as bs eq).product bs).map (fun (f, b) a' => if eq a a' then b else f a') :=
+  rfl
 
--- theorem beq.enumerate_correct : Complete (enumerate t) :=
---   match t with
---   | .unit => fun () => List.mem_singleton_self ()
---   | .bool => fun
---     | true => List.mem_cons_self
---     | false => List.mem_cons_of_mem true (List.mem_singleton_self false)
---   | .pair _ _ => fun (y₁, y₂) =>
---       List.mem_product.mpr ⟨beq.enumerate_correct y₁, beq.enumerate_correct y₂⟩
---   | .fn _ _ => beq.enumerateFn_correct beq.enumerate_correct
+theorem enumerateArrow_ne_nil (hb : bs ≠ []) : enumerateArrow as bs eq ≠ [] :=
+  match as with
+  | [] => match bs with | _ :: _ => List.cons_ne_nil _ _
+  | _ :: _ => fun hn =>
+    have hn := List.map_eq_nil_iff.mp hn
+    have := List.product_ne_nil (enumerateArrow_ne_nil hb (eq := eq)) hb
+    this hn
 
--- theorem eq_of_beq_eq_true (h : beq t x y) : x = y :=
---   match t with
---   | .unit => rfl
---   | .bool => LawfulBEq.eq_of_beq h
---   | .pair _ _ =>
---     have ⟨h₁, h₂⟩ := Bool.and_eq_true_iff.mp h
---     Prod.mk.injEq .. ▸ ⟨eq_of_beq_eq_true h₁, eq_of_beq_eq_true h₂⟩
---   | .fn _ _ =>
---     funext fun arg =>
---       eq_of_beq_eq_true <|
---         List.all_eq_true.mp h arg (beq.enumerate_correct arg)
+theorem enumerate_ne_nil : enumerate t ≠ [] :=
+  match t with
+  | .unit | .bool => List.cons_ne_nil _ _
+  | .pair _ _ => List.product_ne_nil enumerate_ne_nil enumerate_ne_nil
+  | .arrow _ _ => enumerateArrow_ne_nil enumerate_ne_nil
 
--- instance {t : Finite} : LawfulBEq t.asType where
---   rfl := beq_refl
---   eq_of_beq := eq_of_beq_eq_true
+theorem beq_refl : beq t x x = true :=
+  match t with
+  | .unit => rfl
+  | .bool => match x with | true | false => rfl
+  | .pair _ _ => Bool.and_eq_true_iff.mpr ⟨beq_refl, beq_refl⟩
+  | .arrow _ _ => List.all_eq_true.mpr fun _ _ => beq_refl
+
+abbrev _root_.Complete (l : List α) : Prop :=
+  ∀ a, a ∈ l
+
+section
+
+-- theorem enumerateArrow_bij_left {as : List α} {bs : List β} (f : α → α') {eq : α → α → Bool} (hf : Functio)
+    -- enumerateArrow (as.map f) bs eq' = enumerateArrow as bs eq
+
+-- theorem enumerateArrow_map_right {as : List α} {bs : List β} (f : β → β') {eq : α → α → Bool} :
+--     enumerateArrow as (bs.map f) eq = (enumerateArrow as bs eq).map (f ∘ ·) :=
+--   match as with
+--   | [] => match bs with | [] | _ :: _ => rfl
+--   | a :: as' => by
+--     simp only [enumerateArrow_cons, List.map_map]
+--     rw [enumerateArrow_map_right, ←List.map_product]
+--     rw [List.map_map]
+--     unfold Prod.map
+--     unfold Function.comp
+--     dsimp
+--     congr 1
+--     funext (f', b) a'
+--     match eq a a' with | true => rfl | false => rfl
+--     -- TODO: cleanup
+
+theorem enumerateArrow_mem_attach_mp {as : List α} {bs : List β} {eq : α → α → Bool} (ha : Complete as):
+    ∀ (f : α → β), (f ·.1) ∈ enumerateArrow as.attach bs (eq · ·) → f ∈ enumerateArrow as bs eq := by
+  -- TODO lmao clean this up
+  unfold enumerateArrow
+  simp
+  intro f h
+  let r : List ({ x // x ∈ as } → β) → List (α → β) → Prop :=
+    fun l' l => ∀ f, (f ·.1) ∈ l' → f ∈ l
+
+  have h' := @List.foldr_subtype α (β := List ({ x // x ∈ as } → β)) (p := (· ∈ as)) (as.attach) (fun a acc => List.map (fun x a' => if eq a.val a'.val = true then x.snd else x.fst a') (acc.product bs))
+      (fun a acc => List.map (fun x a' => if eq a a'.val then x.snd else x.fst a') (acc.product bs))
+  rw [h' (by simp), List.unattach_attach] at h
+  -- show r _ _
+  -- rw [List.foldr_attach (f := (fun a acc => List.map (fun (f', b) a' => if eq a a'.val = true then b else f' a') (acc.product bs)))] at h
+  --  (r := r)
+
+  revert h
+  -- apply List.foldr_rel
+  revert f
+  show r _ _
+  apply List.foldr_rel
+  · intro f
+    match bs with
+    | [] => simp
+    | _ :: _ => simp; intro h; funext a; have := congrFun h ⟨a, ha a⟩; simp [this]
+  · intro a _ fs' fs h
+    -- simp
+    -- have : (fs'.product bs).map (fun (f, b) (a' : { x // x ∈ as }) => if eq a a'.val then b else f a')
+    --      = (fs.product bs).map  (fun (f, b) (a' : _)               => if eq a a'.val then b else f a') :=
+
+    --   have := h sorry
+    --   sorry
+    intro f hf
+    rw [List.mem_map] at ⊢ hf
+    have ⟨(f', b), hmem, heq'⟩ := hf
+
+    have ⟨hf', hb⟩ := List.mem_product.mp hmem
+    exists ((f' ⟨·, ha _⟩), b)
+    rewrite [List.mem_product]
+    simp at heq'
+    have heq'' : f = fun a' => if eq a a' then b else f' ⟨a', ha a'⟩ := by
+      funext a'
+      let a'' := Subtype.mk a' (ha a')
+      have : a' = a''.val := rfl
+      rw [this, ←congrFun heq' a'']
+    refine ⟨⟨?_, ?_⟩, ?_⟩
+    · apply h
+      simp
+      exact hf'
+    · assumption
+    · funext a'
+      let a'' : {a // a ∈ as} := ⟨a', ha a'⟩
+      rw [heq'']
+
+--   match as with
+--   | [] =>
+--     match bs with
+--     | [] => simp [enumerateArrow] at h
+--     | _ :: _ => exact List.mem_singleton.mpr <| funext fun a => nomatch (ha a)
+--   | a :: as' =>
+--     simp [enumerateArrow_cons]
+--     exists f, f a
+--     rw [List.mem_product]
+--     refine ⟨⟨?_, ?_⟩, ?_⟩
+--     · have := enumerateArrow_mem_attach_mp (as := as'.attach) (eq := (eq · ·)) (by simp_all) as'.mem_attach hb (f ·)
+--       sorry
+--     · apply hb
+--     · funext a <;> simp_all
+-- termination_by as.length
+
+theorem enumerateArrow_complete {α β} (as : List α) {bs : List β} (hb : bs ≠ []) {eq : α → α → Bool} (heq : ∀ a a', eq a a' = true ↔ a = a')
+    (ha : Complete as) (hb' : Complete bs)
+    :
+    Complete (enumerateArrow as bs eq) :=
+  match as with
+  | [] => match bs with | b :: bs' => fun f =>
+    List.mem_singleton.mpr <| funext fun a => nomatch (ha a)
+    --List.attach_nil ▸ List.mem_singleton.mpr (funext nofun)
+  | a :: as' => by
+    simp [enumerateArrow_cons, Complete]
+    show ∀ f, ∃ f' b', _
+    intro f
+    exists f, f a
+    rw [List.mem_product]
+    refine ⟨⟨?_, ?_⟩, ?_⟩
+    ·
+      have := enumerateArrow_complete as'.attach hb (eq := (eq · ·)) (by simp_all) as'.mem_attach hb' (f ·)
+      simp at this
+      unfold enumerateArrow at this
+      simp at this
+      have h' := @List.foldr_subtype α (β := List ({ x // x ∈ as' } → β)) (p := (· ∈ as')) (as'.attach) (fun a acc => List.map (fun x a' => if eq a.val a'.val = true then x.snd else x.fst a') (acc.product bs))
+        (fun a acc => List.map (fun x a' => if eq a a'.val then x.snd else x.fst a') (acc.product bs))
+      rw [h' (by simp)] at this
+      simp at this
+      unfold enumerateArrow
+      simp
+
+      sorry
+      -- rw [List.foldr_subtype (g := fun (a : α) acc => List.map (fun x a' => if eq a a'.val = true then x.snd else x.fst a'))] at this
+      -- · sorry
+      -- · sorry
+      -- · exact fun _ => id
+    · apply hb'
+    · funext a'
+      simp [heq]
+      intro ha'; subst a; rfl
+
+termination_by as.length
+      --have := enumerateArrow_complete as' (bs := b :: bs') hb (eq := eq) heq
+      --simp [enumerateArrow_cons, Complete, List.mem_product] at ⊢ this
+      --
+      -- intro f
+      -- exists f, sorry
+      -- refine have h := ?_; ⟨⟨?_, h⟩, h, ?_⟩
+      -- · rw [←List.mem_cons]
+      --   apply (f _).property
+      -- ·
+      --   have := this (fun ⟨x, hx⟩ => f ⟨x, by simp [hx]⟩)
+      --   simp at this
+      --   simp [List.map_attach_eq_pmap]
+      --   -- rw [List.attach, List.attachWith, List.map_pmap]
+      --   -- rw [List.attach, List.attachWith, List.map_pmap]
+
+      --   sorry
+      -- · funext; simp_all
+
+  -- match as, bs with
+  -- | a :: as', [] => fun f => nomatch (f ⟨a, List.mem_cons_self⟩)
+  -- | a :: as', b :: bs' => fun f => by
+  --   have := enumerateArrow_complete (a :: as') ha bs' eq f
+  --   simp only [List.attach_cons, enumerateArrow_cons, List.mem_map]
+  --   simp
+  --   sorry
+
+end
+
+mutual
+
+theorem eq_of_beq_eq_true (h : beq t x y = true) : x = y :=
+  match t with
+  | .unit => rfl
+  | .bool => LawfulBEq.eq_of_beq h
+  | .pair _ _ =>
+    have ⟨h₁, h₂⟩ := Bool.and_eq_true_iff.mp h
+    Prod.mk.injEq .. ▸ ⟨eq_of_beq_eq_true h₁, eq_of_beq_eq_true h₂⟩
+  | .arrow _ _ =>
+    funext fun arg =>
+      eq_of_beq_eq_true <|
+        List.all_eq_true.mp h arg (enumerate_complete arg)
+
+theorem enumerate_complete : Complete (enumerate t) :=
+  match t with
+  | .unit => fun () => List.mem_singleton_self ()
+  | .bool => fun
+    | true => List.mem_cons_self
+    | false => List.mem_cons_of_mem true (List.mem_singleton_self false)
+  | .pair _ _ => fun (y₁, y₂) =>
+    List.mem_product.mpr ⟨enumerate_complete y₁, enumerate_complete y₂⟩
+  | .arrow tα tβ => sorry
+end
+
+instance {t : Finite} : LawfulBEq t.asType where
+  rfl := beq_refl
+  eq_of_beq := eq_of_beq_eq_true
+#check List.recOn
